\textbf{proof}\\
Let consider the Hadamard walk. In this case,
$$ U(k) = \frac{1}{\sqrt{2}}\begin{bmatrix}
    e^{ik} & e^{ik}\\
    e^{-ik} & -e^{-ik}
\end{bmatrix}$$

The eigenvalues are 
$$
\lambda_1(k) = \frac{1}{\sqrt{2}}(\sqrt{I} + isin(k))
$$\\
$$
\lambda_2(k) = \frac{1}{\sqrt{2}}(-\sqrt{I} + isin(k))
$$
where I = 1 + cos^2(k). Then\\
\begin{center}
    $h_1(k) = \dfrac{D\lambda_1(k)}{\lambda_1(k)} = -\dfrac{cos k}{\sqrt{I}}, h_2(k) = \dfrac{D\lambda_2(k)}{\lambda_2(k)} = \dfrac{cos k}{\sqrt{I}}$
\end{center}
 
\\
where $ D = \dfrac{id}{dk}$.
\\